WIP

extraction/theories/EnvEval.v
@@ -2,100 +2,370 @@ From Coq Require Import List.
 From ConCert.Extraction Require Import ClosedAux.
 From ConCert.Extraction Require Import Utils.
 From ConCert.Extraction Require Import WcbvEvalAux.
+From Equations Require Import Equations.
 From MetaCoq.Erasure Require Import EAst.
 From MetaCoq.Erasure Require Import EAstUtils.
+From MetaCoq.Erasure Require Import EInduction.
 From MetaCoq.Erasure Require Import ELiftSubst.
 From MetaCoq.Erasure Require Import ECSubst.
 From MetaCoq.Erasure Require Import ETyping.
 From MetaCoq.Erasure Require Import EWcbvEval.
 From MetaCoq.Template Require Import utils.
+From MetaCoq.PCUIC Require PCUICAstUtils.
+
+Set Keyed Unification.
 
 Import ListNotations.
 
 Section env_eval.
-  Context {wfl : WcbvFlags}.
+  Reserved Notation "Σ ;;; σ 'e⊢' t , args ▷ v" (at level 50, σ, t, v at next level).
 
-  Reserved Notation "Σ ;;; σ 'e⊢' t ▷ v" (at level 50, σ, t, v at next level).
+  Definition is_stuck_fix (defs : mfixpoint term) (i nargs : nat) :=
+    match nth_error defs i with
+    | Some def => nargs <=? rarg def
+    | None => false
+    end.
 
-  Inductive env_eval (Σ : global_declarations) (σ : list term) : term -> term -> Type :=
+  (*
+  Inductive ee_val : Type :=
+  | vLambda (na : name) (body : term)
+  | vFix (defs : mfixpoint term) (idx : nat
+
+  Inductive ee_val : term -> Type :=
+  | vLambda
+      (na : name) (body : term)
+      (σ : list term) (σv : All ee_val σ) : ee_val (tLambda na body)
+  | vFix
+      (defs : mfixpoint term)
+      (idx : nat)
+      (σ : list term) (σv : All ee_val σ)
+      (args : list term) (argsv : All ee_val args)
+      (is_stuck : is_stuck_fix defs idx #|args|) : ee_val (tFix defs idx)
+  | vBox : ee_val tBox
+  | vConstruct ind c args (argsv : All ee_val args) : ee_val (tConstruct ind c)
+  | vCoFix defs i args (argsv : All ee_val args) : ee_val (tCoFix defs i).
+
+  Definition ee_val_sig := ∑ t, ee_val t.
+*)
+
+  Inductive ee_val : Type :=
+  | vLambda
+      (na : name)
+      (body : term)
+      (σ : list ee_val)
+  | vFix
+      (mfix : mfixpoint term)
+      (idx : nat)
+      (σ : list ee_val)
+      (args : list ee_val)
+  | vCoFix
+      (mfix : mfixpoint term)
+      (idx : nat)
+      (σ : list ee_val)
+      (args : list ee_val)
+  | vBox
+  | vConstruct (ind : inductive) (c : nat) (args : list ee_val).
+
+  Derive NoConfusion NoConfusionHom for ee_val.
+
+  Definition env_fixes mfix σ :=
+    let fix aux n :=
+        match n with
+        | 0 => []
+        | S n => vFix mfix n σ [] :: aux n
+        end in
+    aux #|mfix|.
+
+  Lemma env_fixes_length mfix σ :
+    #|env_fixes mfix σ| = #|mfix|.
+  Proof.
+    unfold env_fixes.
+    induction #|mfix|; auto.
+    cbn.
+    f_equal.
+    auto.
+  Qed.
+
+  Definition fix_env (mfix : mfixpoint term) (σ : list ee_val) : list ee_val :=
+    env_fixes mfix σ ++ σ.
+
+  Definition env_cofixes mfix σ :=
+    let fix aux n :=
+        match n with
+        | 0 => []
+        | S n => vCoFix mfix n σ [] :: aux n
+        end in
+    aux #|mfix|.
+
+  Definition cofix_env (mfix : mfixpoint term) (σ : list ee_val) : list ee_val :=
+    env_cofixes mfix σ ++ σ.
+
+  Lemma env_cofixes_length mfix σ :
+    #|env_cofixes mfix σ| = #|mfix|.
+  Proof.
+    unfold env_cofixes.
+    induction #|mfix|; auto.
+    cbn.
+    f_equal.
+    auto.
+  Qed.
+
+  Hint Rewrite env_fixes_length env_cofixes_length : len.
+
+  Inductive env_eval
+            (Σ : global_declarations)
+            (σ : list ee_val) : term -> list ee_val -> ee_val -> Type :=
+  | env_eval_app a av t argsv v :
+      Σ ;;; σ e⊢ a, [] ▷ av ->
+      Σ ;;; σ e⊢ t, (av :: argsv) ▷ v ->
+      Σ ;;; σ e⊢ tApp t a, argsv ▷ v
   | env_eval_rel i v :
       nth_error σ i = Some v ->
-      Σ ;;; σ e⊢ tRel i ▷ v
-  | env_eval_box a t t' :
-      Σ ;;; σ e⊢ a ▷ tBox ->
-      Σ ;;; σ e⊢ t ▷ t' ->
-      Σ ;;; σ e⊢ tApp a t ▷ tBox
-  | env_eval_beta f na b a a' res :
-      Σ ;;; σ e⊢ f ▷ tLambda na b ->
-      Σ ;;; σ e⊢ a ▷ a' ->
-      Σ ;;; (a' :: σ) e⊢ b ▷ res ->
-      Σ ;;; σ e⊢ tApp f a ▷ res
-  | env_eval_zeta na b0 b0' b1 res :
-      Σ ;;; σ e⊢ b0 ▷ b0' ->
-      Σ ;;; (b0' :: σ) e⊢ b1 ▷ res ->
-      Σ ;;; σ e⊢ tLetIn na b0 b1 ▷ res
-  | env_eval_iota ind pars discr c args brs res :
-      Σ ;;; σ e⊢ discr ▷ mkApps (tConstruct ind c) args ->
+      Σ ;;; σ e⊢ tRel i, [] ▷ v
+  | env_eval_box a argsv av :
+      Σ ;;; σ e⊢ a, argsv ▷ vBox ->
+      Σ ;;; σ e⊢ a, (argsv ++ [av]) ▷ vBox
+  | env_eval_beta f argsv na b σ' av res :
+      Σ ;;; σ e⊢ f, argsv ▷ vLambda na b σ' ->
+      Σ ;;; (av :: σ') e⊢ b, [] ▷ res ->
+      Σ ;;; σ e⊢ f, (argsv ++ [av]) ▷ res
+  | env_eval_zeta na val valv body v :
+      Σ ;;; σ e⊢ val, [] ▷ valv ->
+      Σ ;;; (valv :: σ) e⊢ body, [] ▷ v ->
+      Σ ;;; σ e⊢ tLetIn na val body, [] ▷ v
+  | env_eval_iota discr ind pars c argsv brs v :
+      Σ ;;; σ e⊢ discr, [] ▷ vConstruct ind c argsv ->
       is_propositional Σ ind = Some false ->
-      Σ ;;; σ e⊢ iota_red pars c args brs ▷ res ->
-      Σ ;;; σ e⊢ tCase (ind, pars) discr brs ▷ res
-  | env_eval_iota_sing ind pars discr brs n f res :
-      with_prop_case ->
-      Σ ;;; σ e⊢ discr ▷ tBox ->
-      is_propositional Σ ind = Some true ->
-      brs = [(n, f)] ->
-      Σ ;;; σ e⊢ mkApps f (repeat tBox n) ▷ res ->
-      Σ ;;; σ e⊢ tCase (ind, pars) discr brs ▷ res
-  | env_eval_fix f mfix idx argsv a av def res :
-      Σ ;;; σ e⊢ f ▷ mkApps (tFix mfix idx) argsv ->
-      Σ ;;; σ e⊢ a ▷ av ->
+      Σ ;;; σ e⊢ (nth c brs (0, tDummy)).2, (skipn pars argsv) ▷ v ->
+      Σ ;;; σ e⊢ tCase (ind, pars) discr brs, [] ▷ v
+  | env_eval_fix f argsv mfix idx σ' fargsv a av def v :
+      Σ ;;; σ e⊢ f, argsv ▷ vFix mfix idx σ' fargsv ->
+      Σ ;;; σ e⊢ a, [] ▷ av ->
       nth_error mfix idx = Some def ->
-      #|argsv| = rarg def ->
-      Σ ;;; (fix_subst mfix ++ σ) e⊢ tApp (mkApps (dbody def) argsv) av ▷ res ->
-      Σ ;;; σ e⊢ tApp f a ▷ res
-  | env_eval_fix_value f mfix idx argsv a av def :
-      Σ ;;; σ e⊢ f ▷ mkApps (tFix mfix idx) argsv ->
-      Σ ;;; σ e⊢ a ▷ av ->
+      #|fargsv| = rarg def ->
+      Σ ;;; (fix_env mfix σ') e⊢ dbody def, (fargsv ++ [av]) ▷ v ->
+      Σ ;;; σ e⊢ f, (argsv ++ [av]) ▷ v
+  | env_eval_fix_value f argsv mfix idx σ' fargsv a av def :
+      Σ ;;; σ e⊢ f, argsv ▷ vFix mfix idx σ' fargsv ->
+      Σ ;;; σ e⊢ a, [] ▷ av ->
       nth_error mfix idx = Some def ->
-      #|argsv| < rarg def ->
-      Σ ;;; σ e⊢ tApp f a ▷ tApp (mkApps (tFix mfix idx) argsv) av
-  | env_eval_cofix_case ip mfix idx args def brs res :
-      closedn #|σ| (tCoFix mfix idx) ->
+      #|fargsv| < rarg def ->
+      Σ ;;; σ e⊢ f, (argsv ++ [av]) ▷ vFix mfix idx σ' (fargsv ++ [av])
+  | env_eval_cofix_case mfix idx def ind pars args argsv c cargsv brs v :
       nth_error mfix idx = Some def ->
-      Σ ;;; (cofix_subst mfix ++ σ) e⊢ tCase ip (mkApps (dbody def) args) brs ▷ res ->
-      Σ ;;; σ e⊢ tCase ip (mkApps (tCoFix mfix idx) args) brs ▷ res
-  | env_eval_cofix_proj p mfix idx args def res :
-      closedn #|σ| (tCoFix mfix idx) ->
+      All2 (fun t v => Σ ;;; σ e⊢ t, [] ▷ v) args argsv ->
+      Σ ;;; (cofix_env mfix σ) e⊢ dbody def, argsv ▷ vConstruct ind c cargsv ->
+      is_propositional Σ ind = Some false ->
+      Σ ;;; σ e⊢ (nth c brs (0, tDummy)).2, (skipn pars cargsv) ▷ v ->
+      Σ ;;; σ e⊢ tCase (ind, pars) (mkApps (tCoFix mfix idx) args) brs, [] ▷ v
+  (*| env_eval_cofix_proj mfix idx def
       nth_error mfix idx = Some def ->
       Σ ;;; (cofix_subst mfix ++ σ) e⊢ tProj p (mkApps (dbody def) args) ▷ res ->
-      Σ ;;; σ e⊢ tProj p (mkApps (tCoFix mfix idx) args) ▷ res
-  | env_eval_delta c decl body (isdecl : declared_constant Σ c decl) res :
+      Σ ;;; σ e⊢ tProj p (mkApps (tCoFix mfix idx) args) ▷ res*)
+  | env_eval_delta c decl body (isdecl : declared_constant Σ c decl) v :
       cst_body decl = Some body ->
-      closedn #|σ| body ->
-      Σ ;;; σ e⊢ body ▷ res ->
-      Σ ;;; σ e⊢ tConst c ▷ res
-  | env_eval_proj i pars arg discr args res :
-      Σ ;;; σ e⊢ discr ▷ mkApps (tConstruct i 0) args ->
-      is_propositional Σ i = Some false ->
-      Σ ;;; σ e⊢ nth (pars + arg) args tDummy ▷ res ->
-      Σ ;;; σ e⊢ tProj (i, pars, arg) discr ▷ res
-  | env_eval_proj_prop i pars arg discr :
-      with_prop_case ->
-      Σ ;;; σ e⊢ discr ▷ tBox ->
-      is_propositional Σ i = Some true ->
-      Σ ;;; σ e⊢ tProj (i, pars, arg) discr ▷ tBox
-  | env_eval_app_cong f f' a a' :
-      Σ ;;; σ e⊢ f ▷ f' ->
-      negb (isLambda f' || isFixApp f' || isBox f') ->
-      Σ ;;; σ e⊢ a ▷ a' ->
-      Σ ;;; σ e⊢ tApp f a ▷ tApp f' a'
-  | env_eval_atom t :
-      atom t ->
-      closedn #|σ| t ->
-      Σ ;;; σ e⊢ t ▷ t
-  where "Σ ;;; σ 'e⊢' t ▷ v" := (env_eval Σ σ t v) : type_scope.
+      Σ ;;; [] e⊢ body, [] ▷ v ->
+      Σ ;;; σ e⊢ tConst c, [] ▷ v
+  | env_eval_proj discr ind argsv pars arg av :
+      Σ ;;; σ e⊢ discr, [] ▷ vConstruct ind 0 argsv ->
+      is_propositional Σ ind = Some false ->
+      nth_error argsv (pars + arg) = Some av ->
+      Σ ;;; σ e⊢ tProj (ind, pars, arg) discr, [] ▷ av
+  | env_eval_app_construct t argsv ind c cargsv a av :
+      Σ ;;; σ e⊢ t, argsv ▷ vConstruct ind c cargsv ->
+      Σ ;;; σ e⊢ a, [] ▷ av ->
+      Σ ;;; σ e⊢ t, (argsv ++ [av]) ▷ vConstruct ind c (cargsv ++ [av])
+  | env_eval_app_cofix t argsv mfix idx σ' fargsv a av :
+      Σ ;;; σ e⊢ t, argsv ▷ vCoFix mfix idx σ' fargsv ->
+      Σ ;;; σ e⊢ a, [] ▷ av ->
+      Σ ;;; σ e⊢ t, (argsv ++ [av]) ▷ vCoFix mfix idx σ' (fargsv ++ [av])
+  | env_eval_box_atom :
+      Σ ;;; σ e⊢ tBox, [] ▷ vBox
+  | env_eval_lambda_atom na body :
+      Σ ;;; σ e⊢ tLambda na body, [] ▷ vLambda na body σ
+  | env_eval_construct_atom ind c :
+      Σ ;;; σ e⊢ tConstruct ind c, [] ▷ vConstruct ind c []
+  | env_eval_fix_atom mfix idx :
+      Σ ;;; σ e⊢ tFix mfix idx, [] ▷ vFix mfix idx σ []
+  | env_eval_cofix_atom mfix idx :
+      Σ ;;; σ e⊢ tCoFix mfix idx, [] ▷ vCoFix mfix idx σ []
+  where "Σ ;;; σ 'e⊢' t , args ▷ v" := (env_eval Σ σ t args v) : type_scope.
 
-Lemma env_eval_closedn Σ σ t v k :
+  Derive Signature for env_eval.
+
+  Lemma env_eval_forall_list_rect :
+    forall (Σ : global_declarations) (P : list ee_val -> term -> list ee_val -> ee_val -> Type),
+      (forall (σ : list ee_val) (a : term) (av : ee_val) (t : term) (argsv : list ee_val) (v : ee_val),
+          Σ;;; σ e⊢ a, [] ▷ av ->
+                       P σ a [] av -> Σ;;; σ e⊢ t, av :: argsv ▷ v -> P σ t (av :: argsv) v -> P σ (tApp t a) argsv v) ->
+      (forall (σ : list ee_val) (i : nat) (v : ee_val), nth_error σ i = Some v -> P σ (tRel i) [] v) ->
+      (forall (σ : list ee_val) (a : term) (argsv : list ee_val) av,
+          Σ;;; σ e⊢ a, argsv ▷ vBox -> P σ a argsv vBox -> P σ a (argsv ++ [av]) vBox) ->
+      (forall (σ : list ee_val) (f2 : term) (argsv : list ee_val) (na : name)
+              (b : term) (σ' : list ee_val) (av res : ee_val),
+          Σ;;; σ e⊢ f2, argsv ▷ vLambda na b σ' ->
+          P σ f2 argsv (vLambda na b σ') ->
+          Σ;;; (av :: σ') e⊢ b, [] ▷ res -> P (av :: σ') b [] res -> P σ f2 (argsv ++ [av]) res) ->
+      (forall (σ : list ee_val) (na : name) (val : term) (valv : ee_val) (body : term) (v : ee_val),
+          Σ;;; σ e⊢ val, [] ▷ valv ->
+          P σ val [] valv ->
+          Σ;;; (valv :: σ) e⊢ body, [] ▷ v -> P (valv :: σ) body [] v -> P σ (tLetIn na val body) [] v) ->
+      (forall (σ : list ee_val) (discr : term) (ind : inductive) (pars c : nat)
+              (argsv : list ee_val) (brs : list (nat × term)) (v : ee_val),
+          Σ;;; σ e⊢ discr, [] ▷ vConstruct ind c argsv ->
+          P σ discr [] (vConstruct ind c argsv) ->
+          is_propositional Σ ind = Some false ->
+          Σ;;; σ e⊢ (nth c brs (0, tDummy)).2, skipn pars argsv ▷ v ->
+          P σ (nth c brs (0, tDummy)).2 (skipn pars argsv) v -> P σ (tCase (ind, pars) discr brs) [] v) ->
+      (forall (σ : list ee_val) (f5 : term) (argsv : list ee_val) (mfix : mfixpoint term)
+              (idx : nat) (σ' fargsv : list ee_val) (a : term) (av : ee_val) (def0 : def term)
+              (v : ee_val),
+          Σ;;; σ e⊢ f5, argsv ▷ vFix mfix idx σ' fargsv ->
+          P σ f5 argsv (vFix mfix idx σ' fargsv) ->
+          Σ;;; σ e⊢ a, [] ▷ av ->
+          P σ a [] av ->
+          nth_error mfix idx = Some def0 ->
+          #|fargsv| = rarg def0 ->
+          Σ;;; fix_env mfix σ' e⊢ dbody def0, fargsv ++ [av] ▷ v ->
+          P (fix_env mfix σ') (dbody def0) (fargsv ++ [av]) v -> P σ f5 (argsv ++ [av]) v) ->
+      (forall (σ : list ee_val) (f6 : term) (argsv : list ee_val) (mfix : mfixpoint term)
+              (idx : nat) (σ' fargsv : list ee_val) (a : term) (av : ee_val) (def0 : def term),
+          Σ;;; σ e⊢ f6, argsv ▷ vFix mfix idx σ' fargsv ->
+          P σ f6 argsv (vFix mfix idx σ' fargsv) ->
+          Σ;;; σ e⊢ a, [] ▷ av ->
+          P σ a [] av ->
+          nth_error mfix idx = Some def0 ->
+          #|fargsv| < rarg def0 -> P σ f6 (argsv ++ [av]) (vFix mfix idx σ' (fargsv ++ [av]))) ->
+      (forall (σ : list ee_val) (mfix : list (def term)) (idx : nat) (def0 : def term)
+              (ind : inductive) (pars : nat) (args : list term) (argsv : list ee_val)
+              (c : nat) (cargsv : list ee_val) (brs : list (nat × term)) (v : ee_val),
+          nth_error mfix idx = Some def0 ->
+          All2 (fun (t : term) (v0 : ee_val) => Σ;;; σ e⊢ t, [] ▷ v0 × P σ t [] v0) args argsv ->
+          Σ;;; cofix_env mfix σ e⊢ dbody def0, argsv ▷ vConstruct ind c cargsv ->
+          P (cofix_env mfix σ) (dbody def0) argsv (vConstruct ind c cargsv) ->
+          is_propositional Σ ind = Some false ->
+          Σ;;; σ e⊢ (nth c brs (0, tDummy)).2, skipn pars cargsv ▷ v ->
+          P σ (nth c brs (0, tDummy)).2 (skipn pars cargsv) v ->
+          P σ (tCase (ind, pars) (mkApps (tCoFix mfix idx) args) brs) [] v) ->
+      (forall (σ : list ee_val) (c : kername) (decl : constant_body) (body : term),
+          declared_constant Σ c decl ->
+          forall v : ee_val,
+            cst_body decl = Some body ->
+            Σ;;; [] e⊢ body, [] ▷ v ->
+            P [] body [] v -> P σ (tConst c) [] v) ->
+      (forall (σ : list ee_val) (discr : term) (ind : inductive) (argsv : list ee_val)
+              (pars arg : nat) (av : ee_val),
+          Σ;;; σ e⊢ discr, [] ▷ vConstruct ind 0 argsv ->
+          P σ discr [] (vConstruct ind 0 argsv) ->
+          is_propositional Σ ind = Some false ->
+          nth_error argsv (pars + arg) = Some av -> P σ (tProj (ind, pars, arg) discr) [] av) ->
+      (forall (σ : list ee_val) (t : term) (argsv : list ee_val) (ind : inductive)
+              (c : nat) (cargsv : list ee_val) (a : term) (av : ee_val),
+          Σ;;; σ e⊢ t, argsv ▷ vConstruct ind c cargsv ->
+          P σ t argsv (vConstruct ind c cargsv) ->
+          Σ;;; σ e⊢ a, [] ▷ av -> P σ a [] av -> P σ t (argsv ++ [av]) (vConstruct ind c (cargsv ++ [av]))) ->
+      (forall (σ : list ee_val) (t : term) (argsv : list ee_val) (mfix : mfixpoint term)
+              (idx : nat) (σ' fargsv : list ee_val) (a : term) (av : ee_val),
+          Σ;;; σ e⊢ t, argsv ▷ vCoFix mfix idx σ' fargsv ->
+          P σ t argsv (vCoFix mfix idx σ' fargsv) ->
+          Σ;;; σ e⊢ a, [] ▷ av -> P σ a [] av -> P σ t (argsv ++ [av]) (vCoFix mfix idx σ' (fargsv ++ [av]))) ->
+      (forall σ : list ee_val, P σ tBox [] vBox) ->
+      (forall (σ : list ee_val) (na : name) (body : term), P σ (tLambda na body) [] (vLambda na body σ)) ->
+      (forall (σ : list ee_val) (ind : inductive) (c : nat),
+          P σ (tConstruct ind c) [] (vConstruct ind c [])) ->
+      (forall (σ : list ee_val) (mfix : mfixpoint term) (idx : nat),
+          P σ (tFix mfix idx) [] (vFix mfix idx σ [])) ->
+      (forall (σ : list ee_val) (mfix : mfixpoint term) (idx : nat),
+          P σ (tCoFix mfix idx) [] (vCoFix mfix idx σ [])) ->
+      forall (σ : list ee_val) (t : term) (l : list ee_val) (e : ee_val), Σ;;; σ e⊢ t, l ▷ e -> P σ t l e.
+  Proof.
+    intros until 18.
+    fix f 5.
+    intros σ t l e ev.
+    move f at top.
+    destruct ev;
+      try solve [multimatch goal with
+                 | [H: _ |- _] => eapply H; eauto
+                 end].
+    eapply X7; eauto.
+    clear -a f.
+    revert args argsv a.
+    fix f' 3.
+    intros args argsv [].
+    - apply All2_nil.
+    - constructor.
+      + split; [exact e|].
+        apply f.
+        exact e.
+      + apply f'.
+        exact a.
+  Defined.
+
+  Inductive full_ee_val : ee_val -> Type :=
+  | fvLambda na body σ :
+      All full_ee_val σ ->
+      full_ee_val (vLambda na body σ)
+  | fvFix mfix idx σ args def :
+      nth_error mfix idx = Some def ->
+      All full_ee_val σ ->
+      All full_ee_val args ->
+      #|args| <= rarg def ->
+      full_ee_val (vFix mfix idx σ args)
+  | fvCoFix mfix idx σ args :
+      All full_ee_val σ ->
+      All full_ee_val args ->
+      full_ee_val (vCoFix mfix idx σ args)
+  | fvBox : full_ee_val vBox
+  | fvConstruct ind c args :
+      All full_ee_val args ->
+      full_ee_val (vConstruct ind c args).
+
+  Derive Signature NoConfusion for full_ee_val.
+
+  (*
+  Lemma env_eval_to_value Σ σ t args v :
+    Σ ;;; σ e⊢ t, args ▷ v ->
+    All full_ee_val σ ->
+    All full_ee_val args ->
+    full_ee_val v.
+  Proof.
+    intros ev env_val args_val.
+    induction ev using env_eval_forall_list_rect; auto.
+    - eapply nth_error_all in env_val; eauto.
+    - apply IHev2; auto.
+      apply All_app in args_val as (?&?).
+      depelim a0.
+      constructor; auto.
+      do 2 forward IHev1 by auto.
+      depelim IHev1.
+      auto.
+    - apply IHev2; auto.
+      do 2 forward IHev1 by auto.
+      depelim IHev1.
+      now apply All_skipn.
+    - apply All_app in args_val as (?&?).
+      do 2 forward IHev1 by auto.
+      depelim IHev1.
+      apply IHev3; auto.
+      + admit.
+      + apply All_app_inv; auto.
+    - depelim args_val.
+      econstructor; eauto.
+      + do
+*)
+
+  Fixpoint term_of_ee_val (e : ee_val) : term :=
+    match e with
+    | vLambda na body σ => subst (map term_of_ee_val σ) 0 (tLambda na body)
+    | vFix mfix idx σ args => mkApps (subst (map term_of_ee_val σ) 0 (tFix mfix idx))
+                                     (map term_of_ee_val args)
+    | vBox => tBox
+    | vConstruct ind c args => mkApps (tConstruct ind c) (map term_of_ee_val args)
+    | vCoFix mfix idx σ args => mkApps (subst (map term_of_ee_val σ) 0 (tCoFix mfix idx))
+                                       (map term_of_ee_val args)
+    end.
+
+(*Lemma env_eval_closedn Σ σ t v k :
   Σ ;;; σ e⊢ t ▷ v ->
   env_closed Σ ->
   Forall (closedn k) σ ->
@@ -199,8 +469,7 @@ Proof.
   - easy.
   - easy.
   - easy.
-
-
+*)
 
 Ltac facts :=
   repeat
@@ -213,28 +482,307 @@ Ltac facts :=
       assert (closedn k v) by (apply (eval_closedn _ _ _ _ H _ H'); trivial)
     end.
 
-  Lemma env_eval_eval Σ σ t v :
-    env_closed Σ ->
-    closedn #|σ| t ->
-    All value σ ->
-    Σ;;; σ e⊢ t ▷ v ->
-    Σ e⊢ subst σ 0 t ▷ v.
+  Local Existing Instance opt_wcbv_flags.
+
+  Lemma closed_substl s t :
+    All (closedn 0) s ->
+    substl s t = subst0 s t.
   Proof.
-    intros env_clos clos vals ev.
-    induction ev; cbn in *; propify.
-    - rewrite Nat.sub_0_r, e, lift0_id.
+    intros all.
+    induction all in t |- *; cbn.
+    - now rewrite subst_empty.
+    - rewrite (subst_app_decomp [_]).
+      cbn.
+      rewrite lift_closed, closed_subst by auto.
+      auto.
+  Qed.
+
+  Lemma substl_app l l' t :
+    substl (l ++ l') t = substl l' (substl l t).
+  Proof.
+    induction l in t |- *; cbn; auto.
+  Qed.
+
+  (*
+  From MetaCoq.Template Require Import Loader.
+  Unset Guard Checking.
+  MetaCoq Quote Definition foo := (fix f (n : nat) :=
+                                     f n + g n
+                                   with g (n : nat) :=
+                                       0
+                                         for f).
+*)
+  Lemma terms_of_env_fixes mfix σ :
+    map term_of_ee_val (env_fixes mfix σ) =
+    fix_subst (map (map_def (subst (map term_of_ee_val σ) #|mfix|)) mfix).
+  Proof.
+    unfold fix_subst, env_fixes.
+    rewrite map_length.
+    induction #|mfix| at 1 3; auto.
+    cbn.
+    rewrite Nat.add_0_r.
+    f_equal; apply IHn.
+  Qed.
+
+  Lemma terms_of_env_cofixes mfix σ :
+    map term_of_ee_val (env_cofixes mfix σ) =
+    cofix_subst (map (map_def (subst (map term_of_ee_val σ) #|mfix|)) mfix).
+  Proof.
+    unfold cofix_subst, env_cofixes.
+    rewrite map_length.
+    induction #|mfix| at 1 3; auto.
+    cbn.
+    rewrite Nat.add_0_r.
+    f_equal; apply IHn.
+  Qed.
+
+  Lemma env_eval_eval Σ σ t args v :
+    Σ;;; σ e⊢ t, args ▷ v ->
+    Σ e⊢ mkApps (subst (map term_of_ee_val σ) 0 t)
+                (map term_of_ee_val args) ▷ term_of_ee_val v.
+  Proof.
+    intros ev.
+    induction ev using env_eval_forall_list_rect; cbn in *; propify.
+    - eapply eval_mkApps_inv in IHev2 as H; destruct H as (?&?&?&?).
+      eapply eval_mkApps_congr; eauto.
+      eapply eval_tApp_inv in e as H; destruct H as (?&?&?&?).
+      eapply eval_tApp_congr.
+      5: eauto.
+      all: eauto.
       apply value_final.
-      eapply nth_error_all in e; eauto.
-    - destruct clos.
-      eapply eval_box; eauto.
-    - destruct clos.
+      admit.
+    - rewrite Nat.sub_0_r, nth_error_map, H.
+      cbn.
+      rewrite lift0_id.
+      apply value_final.
+      admit.
+    - rewrite map_app, mkApps_app.
+      eapply eval_box; auto.
+      apply value_final.
+      admit.
+    - rewrite map_app, mkApps_app.
+      cbn.
       eapply eval_beta; eauto.
-      facts.
-      assert (closedn #|σ| (tLambda na b)).
-      { eapply eval_closedn.
-        eauto.
-        eauto.
-      apply eval_closed
+      + eapply value_final; admit.
+      + rewrite subst_app_simpl with (l := [_]) in IHev2.
+        cbn in IHev2.
+        rewrite closed_subst; auto.
+        admit.
+    - eapply eval_zeta; eauto.
+      rewrite subst_app_simpl with (l := [_]) in IHev2.
+      cbn in *.
+      rewrite closed_subst; auto.
+      admit.
+    - eapply eval_iota; eauto.
+      unfold iota_red.
+      rewrite nth_map; auto.
+      cbn.
+      rewrite <- map_skipn.
+      auto.
+    - rewrite map_app, mkApps_app in *; cbn in *.
+      eapply eval_fix; eauto.
+      + eapply value_final; admit.
+      + rewrite Nat.add_0_r, map_length.
+        unfold cunfold_fix.
+        rewrite nth_error_map, H.
+        cbn.
+        f_equal.
+        f_equal; eauto.
+        rewrite closed_substl by admit.
+        unfold fix_env.
+        rewrite map_app.
+        cbn.
+        rewrite subst_app_simpl.
+        cbn.
+        autorewrite with len.
+        f_equal.
+        now rewrite terms_of_env_fixes.
+    - rewrite !map_app, !mkApps_app.
+      eapply eval_fix_value.
+      4: rewrite map_length; exact H0.
+      2: apply value_final; admit.
+      2: { unfold cunfold_fix.
+           rewrite nth_error_map, H.
+           cbn.
+           reflexivity. }
+      auto.
+    - rewrite subst_mkApps.
+      cbn.
+      eapply red_cofix_case.
+      + unfold cunfold_cofix.
+        rewrite nth_error_map, H.
+        cbn.
+        reflexivity.
+      + eapply eval_iota.
+        2: auto.
+        2: { unfold iota_red.
+             rewrite nth_map; auto.
+             cbn.
+             rewrite map_skipn in IHev2.
+             eauto. }
+        rewrite closed_substl by admit.
+        unfold cofix_env in IHev1.
+        rewrite map_app, subst_app_simpl in IHev1.
+        autorewrite with len in *.
+        cbn in *.
+        rewrite <- terms_of_env_cofixes.
+        eapply eval_mkApps_inv in IHev1 as H'; destruct H' as (?&_&?&_).
+        eapply eval_mkApps_congr.
+        3: exact e.
+        4: eauto.
+        1: eauto.
+        2: apply All2_map with (g := term_of_ee_val), All2_same.
+        2: intros; apply value_final; admit.
+        apply All2_map.
+        eapply All2_impl; eauto.
+        cbn.
+        intros ? ? (?&?); auto.
+    - eapply eval_delta; eauto.
+      now rewrite subst_empty in IHev.
+    - eapply eval_proj; eauto.
+      rewrite nth_nth_error, nth_error_map, H0.
+      cbn.
+      apply value_final; admit.
+    - rewrite !map_app, !mkApps_app.
+      cbn.
+      eapply eval_app_cong; auto.
+      + rewrite isLambda_mkApps, isFixApp_mkApps, isBox_mkApps; auto.
+      + apply value_final; admit.
+    - rewrite !map_app, !mkApps_app.
+      cbn.
+      eapply eval_app_cong; auto.
+      + rewrite isLambda_mkApps, isFixApp_mkApps, isBox_mkApps; auto.
+      + apply value_final; admit.
+    - eapply eval_atom; auto.
+    - eapply eval_atom; auto.
+    - eapply eval_atom; auto.
+    - eapply eval_atom; auto.
+    - eapply eval_atom; auto.
+  Admitted.
+
+  Lemma env_eval_box_app Σ σ argsv :
+    Σ ;;; σ e⊢ tBox, argsv ▷ vBox.
+  Proof.
+    induction argsv using MCList.rev_ind.
+    - eapply env_eval_box_atom.
+    - eapply env_eval_box; eauto.
+  Qed.
+
+  Lemma env_eval_subst Σ σ t argsv v :
+    Σ ;;; [] e⊢ subst (map term_of_ee_val σ) 0 t, argsv ▷ v ->
+    ∑ v',
+      Σ ;;; σ e⊢ t, argsv ▷ v' × term_of_ee_val v' = term_of_ee_val v.
+  Proof.
+    intros ev.
+    induction t in σ, t, argsv, v, ev |- * using term_forall_list_ind; cbn in *.
+    - depelim ev.
+      + exists vBox.
+        split; auto.
+        eapply env_eval_box_app.
+      + admit.
+      + admit.
+      + admit.
+      + admit.
+      + admit.
+      + admit.
+    - rewrite Nat.sub_0_r in *.
+      rewrite nth_error_map in ev.
+      destruct nth_error eqn:nth; cbn in *.
+      + rewrite lift0_id in ev.
+Lemma env_eval_app_congr Σ σ t args v t' :
+  Σ ;;; σ e⊢ t, args ▷ v ->
+  Σ ;;; σ e⊢ t', args ▷ v
+        exists e.
+        split; [econstructor; eauto|].
+        apply env_eval_eval in ev.
+        cbn in ev.
+        rewrite subst_empty in ev.
+        eapply eval_deterministic; eauto.
+        apply value_final.
+        admit.
+      + rewrite map_length in ev.
+        depelim ev; try solve [destruct argsv; cbn in *; discriminate].
+        rewrite nth_error_nil in e; discriminate.
+    - depelim ev; try solve [destruct argsv; cbn in *; discriminate].
+    - depelim ev; try solve [destruct argsv; cbn in *; discriminate].
+    - depelim ev; try solve [destruct argsv; cbn in *; discriminate].
+      cbn in *.
+      eexists.
+      split.
+      + eapply env_eval_lambda_atom.
+      + cbn.
+        f_equal.
+        now rewrite subst_empty.
+    - depelim ev; try solve [destruct argsv; cbn in *; discriminate].
+      eexists; split.
+      + eapply env_eval_zeta.
+        admit.
+        admit.
+      + admit.
+    - depelim ev; try solve [destruct argsv; cbn in *; discriminate].
+
+    depind ev.
+    - destruct t0; cbn in *; try discriminate.
+      + rewrite Nat.sub_0_r in *.
+        rewrite nth_error_map in H.
+        destruct nth_error eqn:nth; [|discriminate].
+        cbn in *.
+        constructor.
+        rewrite lift0_id in H.
+        destruct e; cbn in *; try discriminate.
+        *
+        econstructor.
+
+  Lemma eval_env_eval' Σ hd args tv :
+    Σ e⊢ mkApps hd args ▷ tv ->
+    ∑ argsv v,
+      All2 (fun a av => Σ ;;; [] e⊢ a, [] ▷ av) args argsv
+      × Σ ;;; [] e⊢ hd, argsv ▷ v
+      × term_of_ee_val v = tv.
+  Proof.
+    intros ev.
+    depind ev.
+    - destruct args as [|? ? _] using MCList.rev_ind.
+      + cbn in *; subst.
+        specialize (IHev1 _ [] _ eq_refl) as (?&?&?&?&?).
+        specialize (IHev2 _ [] _ eq_refl) as (?&?&?&?&?).
+        depelim a0.
+        depelim a1.
+        destruct x0; cbn in *; try discriminate; try solve_discr.
+        exists [], vBox.
+        split; auto.
+        split; auto.
+        eapply env_eval_app; eauto.
+        eapply env_eval_box with (argsv := []).
+        auto.
+      + rewrite mkApps_app in H; cbn in H; noconf H.
+        specialize (IHev1 _ _ _ eq_refl) as (?&?&?&?&?).
+        specialize (IHev2 _ [] _ eq_refl) as (?&?&?&?&?).
+        depelim a0.
+        exists (x ++ [x2]), vBox.
+        split; [apply All2_app; auto|].
+        split; auto.
+        destruct x0; cbn in *; try discriminate; try solve_discr.
+        eapply env_eval_box.
+        auto.
+    - destruct args as [|? ? _] using MCList.rev_ind.
+      + cbn in *; subst.
+        specialize (IHev1 _ [] _ eq_refl) as (?&?&?&?&?).
+        specialize (IHev2 _ [] _ eq_refl) as (?&?&?&?&?).
+        specialize (IHev3 _ [] _ eq_refl) as (?&?&?&?&?).
+        depelim a0.
+        depelim a1.
+        depelim a2.
+        destruct x0; cbn in *; try discriminate; try solve_discr.
+        noconf e0.
+        eexists [], _.
+        split; auto.
+        exists [], x4.
+        split; auto.
+        split; auto.
+        eapply env_eval_app; eauto.
+        eapply env_eval_beta with (argsv := []); eauto.
+        noconf e0.
 
 
 End env_eval.
